Changes to Spanning_Trees

Spanning_Trees/Kruskal_Greedy.thy
@@ -1,36 +1,852 @@
 theory Kruskal_Greedy
-  imports Matroids_Greedy.Best_In_Greedy Spanning_Trees
+  imports Matroids_Greedy.Best_In_Greedy Spanning_Trees Graph_Algorithms.DFS_Cycles_Aux
+    Graph_Algorithms.DFS_Cycles Insertion_Sort_Desc Graphs_Matroids_Encoding
+    "HOL-Data_Structures.Set2_Join_RBT" "HOL-Data_Structures.RBT_Map" "HOL-Library.Product_Lexorder"
 begin
 
+(* TODO can remove this *)
 context graph_abs
 begin
 
-(* Cycle matroid on undirected graphs (TODO maybe put this in Spanning_Trees file) *)
 interpretation graph_matroid: matroid
   where carrier = "G" and indep = has_no_cycle
-  apply standard
-  using finite_E has_no_cycle_indep_subset_carrier has_no_cycle_indep_ex has_no_cycle_indep_subset 
-    has_no_cycle_augment
-  by blast+
+  using graph_matroid by blast
 
-(* TODO put stuff here in spanning tree file *)
+thm is_spanning_forest_def
+print_interps matroid
 
-(* For showing that basis wrt has_no_cycle is spanning tree: *)
-thm "graph_matroid.basis_def"
-(* Need to show that (\<forall>x\<in>G - ?X. \<not> has_no_cycle (insert x ?X)) is equivalent to the fact that
-every pair of vertices is connected by a walk 
-If {v, w} is in G v and w are obviously connected by a walk
+thm graph_matroid.basis_def
 
-We should have a theorem:
-If X does not contain a cycle but (insert {v, w} X) contains a cycle, there is a walk between
-v and w (this is one direction of thm, basis imp connected)
-\<Rightarrow> should almost be given by decycle_edge_path, along with some reasoning in insert_edge_cycle_ex_walk_betw
+thm spanning_forest_iff_basis
 
-Other direction of thm (connected imp basis):
-need smth like
-  "X \<subseteq> G \<Longrightarrow> \<exists>p. walk_betw X v p w \<Longrightarrow> {v, w} \<notin> X \<Longrightarrow> \<exists>u c. decycle (insert {v, w} X) u c"
+end
 
-\<Longrightarrow> Should be able to just use contrapositive of has_no_cycle_ex_unique_path
+(* Should connecting stuff go in separate file + locale? How to do this *)
+
+(* TODO NOW first probably put all instantiations here *)
+
+subsection \<open>Instantiations for Kruskal's algorithm\<close>
+
+(* TODO IMPORTANT MAKE SURE ALL TYPES ARE CORRECT (ESPECIALLY SINCE WE WILL HAVE
+SET DATATYPE FOR BOTH PAIR GRAPH AND FOR CUSTOM SET *)
+
+(* \<Longrightarrow> We will have vertex type 'v (probably with linorder) assumption, rest will be based on this
+(for pair graph we will have 'v being 'v, 'neighb being tree of 'v, 'adj tree of trees 
+
+For custom set implementation: will probably define uEdge 'v (as quotient type with unequal elements)
+
+\<Rightarrow> Potential problem: Does type class instantiation work in context? \<Rightarrow> How will we instantiate
+uEdge as linorder?
+*)
+
+
+
+
+(*
+type_synonym 'v vertex_rbt = "('v \<times> color) tree"
+
+term "\<langle>\<rangle>::('v rbt)"
+*)
+(* IMPORTANT: DO WE NEED TO SPECIFY EVERYTHING RELEVANT WITH ('v::linorder) or not? *)
+
+abbreviation "rbt_inv \<equiv> \<lambda>t. (invc t \<and> invh t) \<and> Tree2.bst t"
+
+fun rbt_sel where
+  "rbt_sel Leaf = undefined"
+| "rbt_sel (Node _ (a,_) _) = a"
+
+lemma rbt_sel_correct:
+  "t \<noteq> empty \<Longrightarrow> rbt_sel t \<in> (set o inorder) t"
+  by (induction t) (auto simp: empty_def)
+
+interpretation Set_Choose_RBT: Set_Choose
+  where empty = "\<langle>\<rangle>" and insert = insert_rbt and delete = delete_rbt and
+    isin = isin and t_set = "Tree2.set_tree" and invar = "rbt_inv::(('v::linorder) rbt \<Rightarrow> bool)" and
+    sel = rbt_sel
+  apply(simp add: Set_Choose_def)
+  apply(intro conjI)
+  subgoal
+    using RBT.Set_axioms[unfolded] by(auto simp add: S.set_def S.invar_def)
+  subgoal apply unfold_locales subgoal for s by (cases s) (auto dest!: rbt_sel_correct)
+  done
+  done
+
+(* Should we just do Pair_Graph_U or also Pair_Graph? *)
+interpretation Pair_Graph_U_RBT: Pair_Graph_U_Specs
+  where empty = RBT_Set.empty and update = update and delete = RBT_Map.delete and
+    lookup = lookup and adj_inv = "M.invar" and neighb_empty = "\<langle>\<rangle>" and
+    insert = insert_rbt and neighb_delete = delete_rbt and neighb_inv = "rbt_inv::(('v::linorder) rbt \<Rightarrow> bool)" and
+    isin = isin and t_set = "Tree2.set_tree" and sel = rbt_sel
+  apply(simp add: Pair_Graph_U_Specs_def Pair_Graph_Specs_def)
+  using M.Map_axioms Set_Choose_RBT.Set_Choose_axioms by simp
+
+interpretation DFS_Aux_Interp: DFS_Aux
+  where empty = RBT_Set.empty and update = update and delete = RBT_Map.delete and
+    lookup = lookup and adj_inv = "M.invar" and neighb_empty = "\<langle>\<rangle>" and
+    insert = insert_rbt and neighb_delete = delete_rbt and neighb_inv = "rbt_inv::(('v::linorder) rbt \<Rightarrow> bool)" and
+    isin = isin and t_set = "Tree2.set_tree" and union = "RBT.union" and inter = "RBT.inter" and 
+    diff = "RBT.diff" and sel = rbt_sel for G and s
+  apply(simp add: DFS_Aux_def)
+  using Pair_Graph_U_RBT.Pair_Graph_Specs_axioms RBT.Set2_axioms by auto
+
+abbreviation "DFS_Aux' G s \<equiv> DFS_Aux_Interp.DFS_Aux G (DFS_Aux_Interp.initial_state s)"
+
+interpretation DFS_Cycles_Interp: DFS_Cycles
+  where empty = RBT_Set.empty and update = update and delete = RBT_Map.delete and
+    lookup = lookup and adj_inv = "M.invar" and neighb_empty = "\<langle>\<rangle>" and
+    insert = insert_rbt and neighb_delete = delete_rbt and neighb_inv = "rbt_inv::(('v::linorder) rbt \<Rightarrow> bool)" and
+    isin = isin and t_set = "Tree2.set_tree" and union = "RBT.union" and inter = "RBT.inter" and 
+    diff = "RBT.diff" and sel = rbt_sel and seen_aux = "DFS_Aux_state.seen" and cycle_aux = "DFS_Aux_state.cycle" and
+    dfs_aux = "DFS_Aux' G" for G and V
+  apply(simp add: DFS_Cycles_def)
+  using Pair_Graph_U_RBT.Pair_Graph_Specs_axioms RBT.Set2_axioms by auto
+
+lemma DFS_Aux_correct_1_inst:
+  assumes "DFS_Cycles.DFS_Cycles_axioms isin Tree2.set_tree M.invar \<langle>\<rangle> rbt_inv lookup G V"
+    "s \<in> dVs (Pair_Graph_U_RBT.digraph_abs G)"
+  shows "DFS_Aux_state.cycle (DFS_Aux' G s) \<Longrightarrow> \<exists>c. cycle' (Pair_Graph_U_RBT.digraph_abs G) c"
+  using assms[simplified DFS_Cycles_Interp.DFS_Cycles_axioms_def[of "G" "V"]]
+    DFS_Aux_Interp.DFS_Aux_correct_1[unfolded DFS_Aux_Interp.DFS_Aux_axioms_def]
+  by blast
+
+lemma DFS_Aux_correct_2_inst:
+  assumes "DFS_Cycles.DFS_Cycles_axioms isin Tree2.set_tree M.invar \<langle>\<rangle> rbt_inv lookup G V"
+    "s \<in> dVs (Pair_Graph_U_RBT.digraph_abs G)"
+  shows "\<not>DFS_Aux_state.cycle (DFS_Aux' G s) \<Longrightarrow>
+    \<nexists>c. cycle' (Pair_Graph_U_RBT.digraph_abs G \<downharpoonright> Tree2.set_tree (DFS_Aux_state.seen (DFS_Aux' G s))) c"
+  using assms[simplified DFS_Cycles_Interp.DFS_Cycles_axioms_def[of "G" "V"]]
+    DFS_Aux_Interp.DFS_Aux_correct_2[unfolded DFS_Aux_Interp.DFS_Aux_axioms_def]
+  by blast
+
+lemma DFS_Aux_correct_3_inst:
+  assumes "DFS_Cycles.DFS_Cycles_axioms isin Tree2.set_tree M.invar \<langle>\<rangle> rbt_inv lookup G V"
+    "s \<in> dVs (Pair_Graph_U_RBT.digraph_abs G)"
+  shows "\<not>DFS_Aux_state.cycle (DFS_Aux' G s) \<Longrightarrow> v \<in> Tree2.set_tree (DFS_Aux_state.seen (DFS_Aux' G s)) \<Longrightarrow>
+    w \<in> dVs (Pair_Graph_U_RBT.digraph_abs G) - Tree2.set_tree (DFS_Aux_state.seen (DFS_Aux' G s)) \<Longrightarrow>
+    \<nexists>p. awalk (Pair_Graph_U_RBT.digraph_abs G) v p w"
+  using assms[simplified DFS_Cycles_Interp.DFS_Cycles_axioms_def[of "G" "V"]]
+    DFS_Aux_Interp.DFS_Aux_correct_3[unfolded DFS_Aux_Interp.DFS_Aux_axioms_def]
+  by blast
+
+lemma DFS_Aux_correct_4_inst:
+  assumes "DFS_Cycles.DFS_Cycles_axioms isin Tree2.set_tree M.invar \<langle>\<rangle> rbt_inv lookup G V"
+    "s \<in> dVs (Pair_Graph_U_RBT.digraph_abs G)"
+  shows "rbt_inv (DFS_Aux_state.seen (DFS_Aux' G s))"
+  using assms[simplified DFS_Cycles_Interp.DFS_Cycles_axioms_def[of "G" "V"]]
+    DFS_Aux_Interp.DFS_Aux_correct_4[unfolded DFS_Aux_Interp.DFS_Aux_axioms_def]
+  by blast
+
+lemma DFS_Aux_correct_5_inst:
+  assumes "DFS_Cycles.DFS_Cycles_axioms isin Tree2.set_tree M.invar \<langle>\<rangle> rbt_inv lookup G V"
+    "s \<in> dVs (Pair_Graph_U_RBT.digraph_abs G)"
+  shows "v \<in> Tree2.set_tree (DFS_Aux_state.seen (DFS_Aux' G s)) \<Longrightarrow>
+    \<exists>p. awalk (Pair_Graph_U_RBT.digraph_abs G) s p v"
+  using assms[simplified DFS_Cycles_Interp.DFS_Cycles_axioms_def[of "G" "V"]]
+    DFS_Aux_Interp.DFS_Aux_correct_5[unfolded DFS_Aux_Interp.DFS_Aux_axioms_def]
+  by blast
+
+lemma DFS_Aux_correct_6_inst:
+  assumes "DFS_Cycles.DFS_Cycles_axioms isin Tree2.set_tree M.invar \<langle>\<rangle> rbt_inv lookup G V"
+    "s \<in> dVs (Pair_Graph_U_RBT.digraph_abs G)"
+  shows "s \<in> Tree2.set_tree (DFS_Aux_state.seen (DFS_Aux' G s))"
+  using assms[simplified DFS_Cycles_Interp.DFS_Cycles_axioms_def[of "G" "V"]]
+    DFS_Aux_Interp.DFS_Aux_correct_6[unfolded DFS_Aux_Interp.DFS_Aux_axioms_def]
+  by blast
+
+
+lemma DFS_Cycles_imp_dfs_aux_axioms:
+  assumes "DFS_Cycles.DFS_Cycles_axioms isin Tree2.set_tree M.invar \<langle>\<rangle> rbt_inv lookup G V"
+  shows "DFS_Cycles.dfs_aux_axioms isin Tree2.set_tree \<langle>\<rangle> rbt_inv lookup G (DFS_Aux' G) DFS_Aux_state.seen DFS_Aux_state.cycle"
+  unfolding DFS_Cycles_Interp.dfs_aux_axioms_def
+  using DFS_Aux_correct_1_inst[OF assms] DFS_Aux_correct_2_inst[OF assms] DFS_Aux_correct_3_inst[OF assms]
+    DFS_Aux_correct_4_inst[OF assms] DFS_Aux_correct_5_inst[OF assms] DFS_Aux_correct_6_inst[OF assms]
+  by meson
+
+
+thm DFS_Cycles_Interp.DFS_Cycles_correct_1
+
+(* If Pair_Graph_U_invar holds + relationship between G and V, we have cycle iff cycle in ugraph_abs *)
+
+abbreviation "DFS_Cycles' G V \<equiv> DFS_Cycles_Interp.DFS_Cycles V G DFS_Cycles_Interp.initial_state"
+
+thm Pair_Graph_U_RBT.pair_graph_u_invar_def
+thm DFS_Cycles.DFS_Cycles_axioms_def
+
+(* Split into multiple statements or not? *)
+lemma DFS_Cycles_correct_final:
+  assumes "Pair_Graph_U_RBT.pair_graph_u_invar G" "rbt_inv V"
+    "Tree2.set_tree (V::(('a::linorder) rbt)) = dVs (Pair_Graph_U_RBT.digraph_abs G)"
+  shows "DFS_Cycles_state.cycle (DFS_Cycles' G V) = (\<exists>u c. decycle (Pair_Graph_U_RBT.ugraph_abs G) u c)"
+proof-
+  have "DFS_Cycles.DFS_Cycles_axioms isin Tree2.set_tree M.invar \<langle>\<rangle> rbt_inv lookup G V"
+    unfolding DFS_Cycles_Interp.DFS_Cycles_axioms_def 
+    using assms[simplified Pair_Graph_U_RBT.pair_graph_u_invar_def[of "G"]]
+      Pair_Graph_U_RBT.digraph_abs_irreflexive[OF assms(1)]
+      Pair_Graph_U_RBT.digraph_abs_symmetric[OF assms(1)] by fastforce
+
+  from DFS_Cycles_Interp.DFS_Cycles_correct_1[OF this DFS_Cycles_imp_dfs_aux_axioms[OF this]]
+    DFS_Cycles_Interp.DFS_Cycles_correct_2[OF this DFS_Cycles_imp_dfs_aux_axioms[OF this]]
+    have "DFS_Cycles_state.cycle (DFS_Cycles' G V) = (\<exists>c. cycle' (Pair_Graph_U_RBT.digraph_abs G) c)"
+    by blast
+  with Pair_Graph_U_RBT.cycle_equivalence[OF assms(1)]
+  show "DFS_Cycles_state.cycle (DFS_Cycles' G V) = (\<exists>u c. decycle (Pair_Graph_U_RBT.ugraph_abs G) u c)"
+    by blast
+qed
+  
+
+
+thm insort_key_desc_stable
+
+(* NOTE: Maybe don't need quotient type but typedef? \<Rightarrow> for making sure that elements of pair are 
+non-equal *)
+(* TODO HOW DOES TYPEDEF WORK? \<Rightarrow> don't need for now, maybe do later
+\<Rightarrow> Also maybe just use uEdge and assume that elements are not equal for now at least *)
+
+value "uEdge True True"
+(*
+definition uEdge_rel :: "('v * 'v) \<Rightarrow> ('v * 'v) \<Rightarrow> bool" where
+  "uEdge_rel = (\<lambda>(u1, v1) (u2, v2). (u1 = u2) \<and> (v1 = v2))"
+
+quotient_type 'v uEdge_quot = "'v * 'v" / "uEdge_rel"
+  morphisms Rep_Integ Abs_Integ
+proof (rule equivpI)
+  show "reflp uEdge_rel" by (auto simp: reflp_def uEdge_rel_def)
+  show "symp uEdge_rel" by (auto simp: symp_def uEdge_rel_def)
+  show "transp uEdge_rel" by (auto simp: transp_def uEdge_rel_def)
+qed
+*)
+
+definition uEdge_rel :: "('v * 'v) \<Rightarrow> ('v * 'v) \<Rightarrow> bool" where
+  "uEdge_rel = (\<lambda>(u1, v1) (u2, v2). {u1, v1} = {u2, v2})"
+
+quotient_type 'v uEdge_quot = "'v * 'v" / "uEdge_rel"
+  morphisms Rep_Integ Abs_Integ
+proof (rule equivpI)
+  show "reflp uEdge_rel" by (auto simp: reflp_def uEdge_rel_def)
+  show "symp uEdge_rel" by (auto simp: symp_def uEdge_rel_def)
+  show "transp uEdge_rel" by (auto simp: transp_def uEdge_rel_def)
+qed
+
+(* NOTE probably don't need quotient type stuff *)
+
+(*
+typedef 'v uedge_new = "{uEdge (a::'v) (b::'v) | a b . a \<noteq> b}"
+  sorry
+*)
+
+(*
+term "(uEdge (0::nat) (1::nat))::(nat uedge_new)"
+
+lemma
+  "(e::('v uedge_new)) = uEdge a b \<Longrightarrow> a \<noteq> b" 
+*)
+
+text \<open>Instantiations for Greedy\<close>
+
+fun rbt_subseteq :: "('a::linorder) rbt \<Rightarrow> 'a rbt \<Rightarrow> bool" where
+  "rbt_subseteq t1 t2 = (case (RBT.diff t1 t2) of Leaf \<Rightarrow> True | _ \<Rightarrow> False)"
+
+lemma rbt_subseteq_correct:
+  "rbt_inv t1 \<Longrightarrow> rbt_inv t2 \<Longrightarrow> (rbt_subseteq t1 t2) = (Tree2.set_tree t1 \<subseteq> Tree2.set_tree t2)"
+  sorry
+
+
+
+
+(* TODO NOW first instantiate everything for Best_In_Greedy (probably just with uEdge for now)
+===> WHAT TO DO ABOUT ASSUMPTION that uEdges elements should not be equal? *)
+
+lemma rbt_size_correct:
+  "rbt_inv X \<longrightarrow> size X = card (Tree2.set_tree X)"
+  sorry
+
+interpretation Custom_Set_RBT: Custom_Set
+  where empty = "\<langle>\<rangle>" and insert = insert_rbt and delete = delete_rbt and invar = "rbt_inv::(('e::linorder) rbt \<Rightarrow> bool)" and
+    isin = isin and set = "Tree2.set_tree" and union = "RBT.union" and inter = "RBT.inter" and diff = "RBT.diff" and
+    subseteq = rbt_subseteq and cardinality = size
+  apply (subst Custom_Set_def)
+  apply(intro conjI)
+  subgoal
+    using RBT.Set2_axioms by blast
+  subgoal
+    apply (subst Custom_Set_axioms_def)
+    using rbt_subseteq_correct rbt_size_correct by blast
+  done
+
+(* NOTE probably won't need this interpretation below, will just be indep function \<Rightarrow> Although do we specify indep 
+function in indep system specs or in matroid? \<Rightarrow> Probably in indep system system specs 
+\<Longrightarrow> TODO Do we need two parameters or not? We have set_of_sets_isin and indep_set
+\<Longrightarrow> TODO NEED TO CONSIDER THIS/ASK 
+Current possible idea: just define set_of_sets_isin as type (('s \<Rightarrow> bool) \<Rightarrow> 's \<Rightarrow> bool) and
+as set_of_sets_isin f a = f a, and then define indep_set as actual independence function with type
+ ('s \<Rightarrow> bool), \<Rightarrow> or alternatively just define one parameter indep_impl as ('s \<Rightarrow> bool), already in
+indep system/matroid, then don't need to specify anything else in Matroids_Greedy
+*)
+
+(* TODO LATER REMOVE UNNECESSARY FUNCTIONS, Set_RBT interpretation *)
+
+definition "set_of_sets_isin f a = f a"
+
+(*
+interpretation Set_RBT: Set
+  where empty = set_of_sets_empty and insert = set_of_sets_insert and delete = set_of_sets_delete and 
+    isin = "set_of_sets_isin :: ('e rbt \<Rightarrow> bool) \<Rightarrow> 'e rbt \<Rightarrow> bool" and set = to_set_of_sets and invar = set_of_sets_inv 
+  apply (subst Set_def)
+  sorry
+*)
+
+interpretation Matroid_Specs_Inst: Matroid_Specs
+  where set_empty = "\<langle>\<rangle>" and set_insert = insert_rbt and set_delete = delete_rbt and set_inv = "rbt_inv::(('e::linorder) rbt \<Rightarrow> bool)" and
+    set_isin = isin and to_set = "Tree2.set_tree" and union = "RBT.union" and inter = "RBT.inter" and diff = "RBT.diff" and
+    subseteq = rbt_subseteq and cardinality = size and
+    set_of_sets_isin = "set_of_sets_isin :: ('e rbt \<Rightarrow> bool) \<Rightarrow> 'e rbt \<Rightarrow> bool"
+  apply (subst Matroid_Specs_def)
+  apply (subst Indep_System_Specs_def)
+  using Custom_Set_RBT.Custom_Set_axioms by blast
+
+
+(* NOW: Just specify 'e::linorder type, instantiate all remaining locales (+ add v1, v2 edge functions
+to encoding locale but not yet assumptions), have final two/three instantianted theorems that greedy
+result is basis/valid solution and matroid opt  
+\<Rightarrow> Need everything which still needs to be instantiated
+LATER: Add necessary assumptions to encoding locale (maybe don't even need this) *)
+
+
+(* IDEA NOW: maybe here in context, just specify 'e :: linorder and assume we have functions v1, v2 which 
+extract vertices from edge, then later (for executing everything on an example) can maybe instantiate
+relevant vertex and edge types as enum with a list, which should also satisfy linorder 
+
+===> HERE just assume v1, v2, edge of functions on arbitrary 'v and 'e types, then instantiate
+with concrete types for executing an example
+\<Rightarrow> satisfy edge_of assumption by defining as follows: if a \<le> b then (a, b) else (b, a)
+\<Rightarrow> for v1_of, v2_of: should v1_of always be first, v2_of always be second?
+((===> OR RATHER just assume vertex type, define functions here with simple pair/uedge!
+\<Rightarrow> Problem: How do we show that edge type itself is of sort linorder? \<Rightarrow> won't work))
+\<Longrightarrow> OR WILL WORK if I import the product linorder stuff
+
+\<Longrightarrow> IMPORTANT: Do I really need assumption that for any edge e, components are non-equal?
+\<Rightarrow> Maybe either remove this assumption or e.g. require this only for a certain set of edges 
+*)
+value "uEdge (3::nat) (4::nat) = uEdge 3 4"
+
+
+(* TODO NOW define indep function with subset check and DFS_Cycles', also need to ! negate ! result
+\<Rightarrow> where does has_no_cycle come into play? *)
+
+term "DFS_Cycles'"
+
+
+(* TODO what about remaining functions? v1, v2, edge *)
+
+
+fun rbt_set_fold :: "'a rbt \<Rightarrow> ('a \<Rightarrow> 'b \<Rightarrow> 'b) \<Rightarrow> 'b \<Rightarrow> 'b" where
+  "rbt_set_fold Leaf f acc = acc"
+| "rbt_set_fold (Node l (a, _) r) f acc = rbt_set_fold r f (f a (rbt_set_fold l f acc))"
+
+fun rbt_map_fold :: "('a \<times> 'd) rbt \<Rightarrow> ('a \<Rightarrow> 'd \<Rightarrow> 'b \<Rightarrow> 'b) \<Rightarrow> 'b \<Rightarrow> 'b" where
+  "rbt_map_fold Leaf f acc = acc"
+| "rbt_map_fold (Node l ((a, d), _) r) f acc = rbt_map_fold r f (f a d (rbt_map_fold l f acc))"
+
+
+interpretation Kruskal_Graphs_Matroids: Graphs_Matroids_Encoding
+  where empty = RBT_Set.empty and update = update and delete = RBT_Map.delete and
+    lookup = lookup and adj_inv = "M.invar" and neighb_empty = "\<langle>\<rangle>" and
+    insert = insert_rbt and neighb_delete = delete_rbt and neighb_inv = "rbt_inv::(('v::linorder) rbt \<Rightarrow> bool)" and
+    isin = isin and t_set = "Tree2.set_tree" and sel = rbt_sel and
+
+    set_empty = "\<langle>\<rangle>" and set_insert = insert_rbt and set_delete = delete_rbt and set_inv = "rbt_inv::(('e::linorder) rbt \<Rightarrow> bool)" and
+    set_isin = isin and to_set = "Tree2.set_tree" and union = "RBT.union" and inter = "RBT.inter" and diff = "RBT.diff" and
+    subseteq = rbt_subseteq and cardinality = size and 
+    set_of_sets_isin = "set_of_sets_isin :: ('e rbt \<Rightarrow> bool) \<Rightarrow> 'e rbt \<Rightarrow> bool" and
+
+    adj_fold = "rbt_map_fold" and neighb_fold = "rbt_set_fold" and set_fold_adj = "rbt_set_fold" and
+    set_fold_neighb = "rbt_set_fold"
+    for v1_of :: "('e::linorder) \<Rightarrow> ('v::linorder)" and v2_of :: "('e::linorder) \<Rightarrow> ('v::linorder)" and 
+        edge_of :: "('v::linorder) \<Rightarrow> 'v \<Rightarrow> ('e::linorder)"
+  apply (subst Graphs_Matroids_Encoding_def)
+  using Pair_Graph_U_RBT.Pair_Graph_U_Specs_axioms Matroid_Specs_Inst.Matroid_Specs_axioms
+  by blast
+
+
+
+
+
+(* TODO Best_In_Greedy instantiation probably needs to be within graph context *)
+
+
+
+(* When formulating final statement: operate in a context fixing a valid graph G or somehow else?
+\<Rightarrow> TODO !! What about c and order? *)
+
+
+
+(*
+thm Pair_Graph_U_RBT.pair_graph_u_invar_def
+term "rbt_inv::(('v::linorder) rbt \<Rightarrow> bool)"
+
+print_interps Pair_Graph_U_Specs
+*)
+
+term Kruskal_Graphs_Matroids.graph_to_edges
+
+(* TODO NOW PUT SOME THINGS OUTSIDE OF CONTEXT (ESP KRUSKAL ITSELF) !! *)
+context
+  fixes input_G :: "(('v::linorder) * ('v rbt)) rbt" and v1_of :: "('e::linorder) \<Rightarrow> 'v"
+    and v2_of :: "('e::linorder) \<Rightarrow> 'v" and edge_of :: "'v \<Rightarrow> 'v \<Rightarrow> 'e"
+  (* assumes pair_graph_u: "Pair_Graph_U_RBT.pair_graph_u_invar graph" *) (* TODO THIS ASSM *)
+begin
+
+(* TODO do we need these two definitions? Maybe just turn into abbreviations? *)
+
+definition Kruskal_E_to_G :: "('e::linorder) rbt \<Rightarrow> ('v \<times> ('v rbt)) rbt" where
+  "Kruskal_E_to_G = Kruskal_Graphs_Matroids.edges_to_graph v1_of v2_of"
+
+definition Kruskal_E_to_V :: "('e::linorder) rbt \<Rightarrow> ('v rbt)" where
+  "Kruskal_E_to_V = Kruskal_Graphs_Matroids.edges_to_vertices v1_of v2_of"
+
+definition carrier_graph_matroid :: "('e::linorder) rbt" where
+  "carrier_graph_matroid \<equiv> Kruskal_Graphs_Matroids.graph_to_edges edge_of input_G"
+
+fun indep_graph_matroid :: "('e::linorder) rbt \<Rightarrow> bool" where
+  "indep_graph_matroid E = 
+    (let
+      G = (Kruskal_E_to_G E);
+      V = (Kruskal_E_to_V E)
+    in
+      (if rbt_subseteq E carrier_graph_matroid then \<not>DFS_Cycles_state.cycle (DFS_Cycles' G V)
+      else False))"
+(* TODO somehow prove this is equivalent to E \<subseteq> carrier \<and> (\<nexists>c u. decycle (ugraph_abs ..)) *)
+(* Also connect implementation and abstract matroid through carrier_abs, indep_abs, etc. *)
+
+(* need to show that carrier_abs of carrier_graph_matroid is ugraph_abs graph
+For this need that to_set graph_to_edges graph = ugraph_abs graph
+
+need to show that indep_abs of indep_graph_matroid is has_no_cycle (ugraph_abs graph)
+given an arbitrary abstract set S: if it is not finite, it obviously cannot satisfy has_no_cycle 
+\<Rightarrow> will evaluate to false
+if it is finite: TODO NOW THINK ABOUT THIS
+\<Rightarrow> will evaluate to
+rbt_subseteq (from_set S) carrier_graph_matroid \<and> 
+  \<not>(\<exists>u c. decycle (Pair_Graph_U_RBT.ugraph_abs (Kruskal_E_to_G (from_set S))) u c))
+
+Need to show that this is equivalent to:
+S \<subseteq> to_set (carrier_graph_matroid) \<and>
+  \<not>(\<exists>u c. decycle 
+
+PROBLEM: ARE WE DEALING WITH TWO REPRESENTATIONS? ABSTRACT SET OF SETS + ABSTRACT SET OF IMPL EDGES?
+\<Longrightarrow> Rather need equivalence between matroid abstractions of implementation and set of sets abstraction
+\<Longrightarrow> Do we need extra functions to convert between abstractions or not?
+
+*)
+
+(* ======== TODO NOW 2/3 things ========
+Think about matroid indep_abs equivalence
+Try instantiating one more of the axioms needed for greedy correctness
+(try to connect everything into final statement (maybe think about cost function properties)
+
+*)
+
+
+
+lemma (* TODO instantiate assms directly using thms from encoding locale, maybe take the statement "further"*)
+  indep_graph_matroid_expr_1:
+  assumes "Pair_Graph_U_RBT.pair_graph_u_invar (Kruskal_E_to_G (E::('e::linorder) rbt))" "rbt_inv (Kruskal_E_to_V E)"
+    "Tree2.set_tree (Kruskal_E_to_V E) = dVs (Pair_Graph_U_RBT.digraph_abs (Kruskal_E_to_G E))"
+  shows "indep_graph_matroid E =
+    (rbt_subseteq E carrier_graph_matroid \<and> \<not>(\<exists>u c. decycle (Pair_Graph_U_RBT.ugraph_abs (Kruskal_E_to_G E)) u c))"
+  apply (subst indep_graph_matroid.simps)
+  apply (subst Let_def)+
+  apply (subst DFS_Cycles_correct_final[OF assms]) by presburger
+
+thm Kruskal_E_to_V_def
+
+lemma
+  indep_graph_matroid_expr_2:
+  assumes "rbt_inv (E::('e::linorder) rbt)"
+  shows "indep_graph_matroid E =
+    (rbt_subseteq E carrier_graph_matroid \<and> \<not>(\<exists>u c. decycle (Pair_Graph_U_RBT.ugraph_abs (Kruskal_E_to_G E)) u c))"
+  using indep_graph_matroid_expr_1[of "E", unfolded Kruskal_E_to_G_def Kruskal_E_to_V_def, OF
+    Kruskal_Graphs_Matroids.edges_invar_imp_graph_invar[OF assms]
+    Kruskal_Graphs_Matroids.edges_invar_imp_vertices_props[OF assms]] 
+  using Kruskal_E_to_G_def by metis
+
+
+
+interpretation Kruskal_Greedy: Best_In_Greedy
+  where set_empty = "\<langle>\<rangle>" and set_insert = insert_rbt and set_delete = delete_rbt and set_inv = "rbt_inv::(('e::linorder) rbt \<Rightarrow> bool)" and
+    set_isin = isin and to_set = "Tree2.set_tree" and union = "RBT.union" and inter = "RBT.inter" and diff = "RBT.diff" and
+    subseteq = rbt_subseteq and cardinality = size and
+    set_of_sets_isin = "set_of_sets_isin :: ('e rbt \<Rightarrow> bool) \<Rightarrow> 'e rbt \<Rightarrow> bool" and 
+    carrier = carrier_graph_matroid and indep_set = indep_graph_matroid and
+    sort_desc = insort_key_desc
+  (* TODO should we instantiate remaining parameters here or just outside? \<Rightarrow> probably should instantiate carrier and indep_set
+  here since they are specified in the locale, but cannot yet instantiate c and order *)
+  apply (subst Best_In_Greedy_def)
+  using Matroid_Specs_Inst.Matroid_Specs_axioms by blast
+
+thm Kruskal_Greedy.BestInGreedy_correct_1
+thm Kruskal_Greedy.BestInGreedy_correct_3
+thm Kruskal_Greedy.BestInGreedy_matroid_iff_opt
+
+(* 
+We have (at least) two cost functions: 
+c from 'v set to rat
+c_imp from 'e to rat
+\<Rightarrow> note: names are not quite consistent with those below
+
+\<Rightarrow> maybe need a third intermediate cost function? the M - ... cost function, but on the abstract type
+
+
+we will have that
+for valid_solution X:
+Kruskal_Greedy.c_set c (Tree2.set_tree X) \<le> 
+  Kruskal_Greedy.c_set c (Tree2.set_tree (result (Kruskal_Greedy.BestInGreedy (Kruskal_Greedy.initial_state c order)))))))
+
+We need to prove that:
+for G' where ugraph_abs G' \<subseteq> ugraph_abs G (+ G' is spanning tree):
+sum c' ugraph_abs G' \<ge>
+ sum c' ugraph_abs (Kruskal_E_to_G (result (Kruskal_Greedy.BestInGreedy (Kruskal_Greedy.initial_state c order))))
+
+Probably need to prove that:
+ugraph_abs G' \<subseteq> ugraph_abs G \<Longrightarrow> valid_solution (Kruskal_E_to_G G') (+ if G' is spanning tree, it is indep wrt function)
+
+we have (assuming E* is result of greedy):
+Kruskal_Greedy.c_set c (Tree2.set_tree (Kruskal_G_to_E G')) \<le> 
+ Kruskal_Greedy.c_set c ( Tree2.set_tree E* )
+\<Longrightarrow>
+Kruskal_Greedy.c_set c (Tree2.set_tree (Kruskal_G_to_E G')) \<le> 
+ Kruskal_Greedy.c_set c (Tree2.set_tree (Kruskal_G_to_E (Kruskal_E_to_G E* ) ))
+\<Longrightarrow> 
+sum c' (ugraph_abs G') \<ge> 
+ sum c' (ugraph_abs (Kruskal_E_to_G E* ))
+
+Either assume last step directly (for two arbitary graphs G1, G2 that one implies the other, or maybe
+somehow show relationship between 
+Kruskal_Greedy.c_set c (Tree2.set_tree (Kruskal_G_to_E G')) and
+sum c' (ugraph_abs G') for arbitrary G'
+\<Rightarrow> Probably that:
+Kruskal_Greedy.c_set c (Tree2.set_tree (Kruskal_G_to_E G')) = 
+card (...) * M - Kruskal_Greedy.c_set ? (Tree2.set_tree (Kruskal_G_to_E G'))
+card (...) * M - sum c' (ugraph_abs G')
+
+TODO think can abstractions be related on a "direct" level?
+e.g. think about the image thing again, what would be two functions which relate elements?
+impl edge to set edge: e \<rightarrow> {v1_of e, v2_of e}
+set edge to impl edge: e', extract v1 and v2 by Hilbert choice \<longrightarrow> edge_of v1 v2
+
+\<Rightarrow> then show that under proper assumptions, it holds that
+Set.image (impl_edge_to_set_edge) (Tree2.set_tree (Kruskal_G_to_E G')) = (ugraph_abs G')
+and/or maybe
+Set.image (set_edge_to_impl_edge) (ugraph_abs (Kruskal_E_to_G E')) = (Tree2.set_tree E')
+
+
+\<Longrightarrow> NOTE: Should M be "hardcoded" or can M be assumed as a parameter (strictly greater than all costs
+within a certain set)
+
+
+*)
+
+term Matroid_Specs_Inst.indep
+term indep_graph_matroid
+
+lemma carrier_graph_matroid_inv:
+  assumes "Pair_Graph_U_RBT.pair_graph_u_invar input_G"
+  shows "rbt_inv carrier_graph_matroid"
+  unfolding carrier_graph_matroid_def
+  using Kruskal_Graphs_Matroids.graph_invar_imp_edges_invar[OF assms] by blast
+
+lemma Kruskal_Greedy_indep':
+  "Kruskal_Greedy.indep' X = indep_graph_matroid X"
+  using Matroid_Specs_Inst.indep_def set_of_sets_isin_def by metis
+
+lemma indep_graph_matroid_abs_equal:
+  assumes "Pair_Graph_U_RBT.pair_graph_u_invar input_G" "rbt_inv X" "rbt_inv Y" "Tree2.set_tree X = Tree2.set_tree Y"
+  shows "indep_graph_matroid X = indep_graph_matroid Y"
+proof-
+  have "rbt_subseteq X carrier_graph_matroid = rbt_subseteq Y carrier_graph_matroid"
+    using rbt_subseteq_correct[OF \<open>rbt_inv X\<close> carrier_graph_matroid_inv[OF assms(1)]]
+    rbt_subseteq_correct[OF \<open>rbt_inv Y\<close> carrier_graph_matroid_inv[OF assms(1)]] assms(4)
+    by blast
+  with Kruskal_Graphs_Matroids.to_set_equal_imp_ugraph_abs_equal[OF assms(2-4)]
+    show "indep_graph_matroid X = indep_graph_matroid Y"
+    apply (subst indep_graph_matroid_expr_2[OF \<open>rbt_inv X\<close>])
+    apply (subst indep_graph_matroid_expr_2[OF \<open>rbt_inv Y\<close>])
+    unfolding Kruskal_E_to_G_def using arg_cong2 .
+qed
+
+lemma Kruskal_BestInGreedy_axioms:
+  assumes "Pair_Graph_U_RBT.pair_graph_u_invar input_G"
+  shows "Best_In_Greedy.BestInGreedy_axioms rbt_inv Tree2.set_tree set_of_sets_isin carrier_graph_matroid indep_graph_matroid"
+  unfolding Kruskal_Greedy.BestInGreedy_axioms_def Matroid_Specs_Inst.invar_def
+    Matroid_Specs_Inst.finite_sets_def
+proof-
+  from carrier_graph_matroid_def Kruskal_Graphs_Matroids.graph_invar_imp_edges_invar[OF assms]
+    have "rbt_inv carrier_graph_matroid" by metis
+
+  with indep_graph_matroid_abs_equal[OF assms] Kruskal_Greedy_indep' finite_set_tree
+    show "(rbt_inv carrier_graph_matroid \<and>
+    (\<forall>X Y. rbt_inv X \<longrightarrow> rbt_inv Y \<longrightarrow> Tree2.set_tree X = Tree2.set_tree Y \<longrightarrow>
+      Kruskal_Greedy.indep' X = Kruskal_Greedy.indep' Y)) \<and>
+    (\<forall>X. finite (Tree2.set_tree X))" by blast
+qed
+
+
+lemma Kruskal_sort_desc_axioms:
+  "Best_In_Greedy.sort_desc_axioms Kruskal_Greedy.carrier_sorted"
+  unfolding Kruskal_Greedy.sort_desc_axioms_def
+  using set_insort_key_desc length_insort_key_desc sorted_desc_f_insort_key_desc insort_key_desc_stable
+  by metis
+
+
+context
+  assumes pair_graph_u: "Pair_Graph_U_RBT.pair_graph_u_invar input_G"
+begin
+
+lemmas carrier_inv = carrier_graph_matroid_inv[OF pair_graph_u]
+
+(*
+interpretation input_G_graph_abs: graph_abs
+  where G = "Pair_Graph_U_RBT.ugraph_abs input_G"
+  using Pair_Graph_U_RBT.graph_abs_ugraph[OF pair_graph_u] by simp
+
+interpretation (Pair_Graph_U_RBT.ugraph_abs (Kruskal_E_to_G carrier_graph_matroid))
+*)
+
+lemma carrier_converted_back:
+  "Kruskal_E_to_G carrier_graph_matroid = input_G"
+  unfolding Kruskal_E_to_G_def carrier_graph_matroid_def 
+  using Kruskal_Graphs_Matroids.graph_to_edges_inverse[OF pair_graph_u] by simp
+
+
+lemma carrier_converted_graph_abs:
+  "graph_abs (Pair_Graph_U_RBT.ugraph_abs (Kruskal_E_to_G carrier_graph_matroid))"
+  using carrier_converted_back Pair_Graph_U_RBT.graph_abs_ugraph[OF pair_graph_u] by metis
+(* Put this into interpretation or not? *)
+
+lemma indep_graph_matroid_expr_3:
+  assumes "rbt_inv (E::('e::linorder) rbt)"
+  shows "indep_graph_matroid E = 
+    graph_abs.has_no_cycle (Pair_Graph_U_RBT.ugraph_abs (Kruskal_E_to_G carrier_graph_matroid))
+    (Pair_Graph_U_RBT.ugraph_abs (Kruskal_E_to_G E))"
+  unfolding graph_abs.has_no_cycle_def[OF carrier_converted_graph_abs]
+  (* (rbt_subseteq E carrier_graph_matroid \<and> \<not>(\<exists>u c. decycle (Pair_Graph_U_RBT.ugraph_abs (Kruskal_E_to_G E)) u c)) *)
+proof-
+  from indep_graph_matroid_expr_2[OF assms]
+  have "indep_graph_matroid E =
+    (rbt_subseteq E carrier_graph_matroid \<and>
+    (\<nexists>u c. decycle (Pair_Graph_U_RBT.ugraph_abs (Kruskal_E_to_G E)) u c))" by blast
+  also have "... = 
+    (Pair_Graph_U_RBT.ugraph_abs (Kruskal_E_to_G E) \<subseteq> Pair_Graph_U_RBT.ugraph_abs (Kruskal_E_to_G carrier_graph_matroid) \<and>
+    (\<nexists>u c. decycle (Pair_Graph_U_RBT.ugraph_abs (Kruskal_E_to_G E)) u c))"
+    unfolding Kruskal_E_to_G_def
+    using Kruskal_Graphs_Matroids.subset_iff_graph_to_edges_subset[OF assms carrier_inv]
+    by (metis Kruskal_Greedy.Kruskal_E_to_G_def carrier_converted_back)
+  finally show "indep_graph_matroid E =
+    (Pair_Graph_U_RBT.ugraph_abs (Kruskal_E_to_G E) \<subseteq> Pair_Graph_U_RBT.ugraph_abs (Kruskal_E_to_G carrier_graph_matroid) \<and>
+     (\<nexists>u c. decycle (Pair_Graph_U_RBT.ugraph_abs (Kruskal_E_to_G E)) u c))" .
+qed
+
+
+(* TODO maybe generalise some parts of these theorems? *)
+
+lemma Kruskal_indep'_eq_has_no_cycle:
+  assumes "rbt_inv (X::('e::linorder) rbt)"
+  shows "Kruskal_Greedy.indep' X = graph_abs.has_no_cycle (Pair_Graph_U_RBT.ugraph_abs (Kruskal_E_to_G carrier_graph_matroid))
+    (Pair_Graph_U_RBT.ugraph_abs (Kruskal_E_to_G X))"
+  using Kruskal_Greedy_indep' indep_graph_matroid_expr_3[OF assms] by blast
+
+lemma Kruskal_indep_subset_carrier:
+  assumes "rbt_inv (X::('e::linorder) rbt)" "Kruskal_Greedy.indep' X"
+  shows "rbt_subseteq X carrier_graph_matroid"
+proof-
+  from assms(2) Kruskal_Greedy_indep' indep_graph_matroid_expr_3[OF assms(1)]
+    have "graph_abs.has_no_cycle (Pair_Graph_U_RBT.ugraph_abs (Kruskal_E_to_G carrier_graph_matroid))
+    (Pair_Graph_U_RBT.ugraph_abs (Kruskal_E_to_G X))" by blast
+  then have "Pair_Graph_U_RBT.ugraph_abs (Kruskal_E_to_G X) \<subseteq>
+    Pair_Graph_U_RBT.ugraph_abs (Kruskal_E_to_G carrier_graph_matroid)"
+    using graph_abs.has_no_cycle_indep_subset_carrier[OF carrier_converted_graph_abs] by blast
+  then have "Tree2.set_tree X \<subseteq> Tree2.set_tree (carrier_graph_matroid)"
+    unfolding Kruskal_E_to_G_def
+    using Kruskal_Graphs_Matroids.edges_to_graph_subset_imp_subset[OF \<open>rbt_inv X\<close> carrier_inv]
+    by auto
+
+  with Custom_Set_RBT.set_subseteq[OF \<open>rbt_inv X\<close> carrier_inv]
+    show "rbt_subseteq X carrier_graph_matroid" by blast
+qed
+
+lemma Kruskal_indep_ex:
+  "(\<exists>X. rbt_inv (X::('e::linorder) rbt) \<and> Kruskal_Greedy.indep' X)"
+proof-
+  from graph_abs.has_no_cycle_indep_ex[OF carrier_converted_graph_abs]
+    obtain G where "graph_abs.has_no_cycle (Pair_Graph_U_RBT.ugraph_abs (Kruskal_E_to_G carrier_graph_matroid)) G"
+    by blast
+  from graph_abs.has_no_cycle_indep_subset_carrier[OF carrier_converted_graph_abs this]
+    have "G \<subseteq> (Pair_Graph_U_RBT.ugraph_abs (Kruskal_E_to_G carrier_graph_matroid))"
+    by (simp add: carrier_converted_back)
+  from graph_abs_mono[OF carrier_converted_graph_abs this]
+    have "graph_abs G" by blast
+  from Pair_Graph_U_RBT.ex_graph_impl_ugraph_abs[OF this]
+    obtain G_impl where G_impl_invar: "Pair_Graph_U_RBT.pair_graph_u_invar G_impl" and
+      G_impl_abs: "Pair_Graph_U_RBT.ugraph_abs G_impl = G"
+    by blast
+
+  (* If G satisfies ugraph_abs, there exists an impl graph satisfying pair_graph_u such that ugraph_abs (G_impl) = *)
+
+  from Kruskal_Graphs_Matroids.graph_invar_imp_edges_invar[OF \<open>Pair_Graph_U_RBT.pair_graph_u_invar G_impl\<close>]
+    have "rbt_inv (Kruskal_Graphs_Matroids.graph_to_edges edge_of G_impl)" .
+
+
+  from \<open>graph_abs.has_no_cycle (Pair_Graph_U_RBT.ugraph_abs (Kruskal_E_to_G carrier_graph_matroid)) G\<close> G_impl_abs
+    have "graph_abs.has_no_cycle (Pair_Graph_U_RBT.ugraph_abs (Kruskal_E_to_G carrier_graph_matroid))
+      (Pair_Graph_U_RBT.ugraph_abs (Kruskal_E_to_G (Kruskal_Graphs_Matroids.graph_to_edges edge_of G_impl)))"
+    unfolding Kruskal_E_to_G_def
+    apply (subst Kruskal_Graphs_Matroids.graph_to_edges_inverse[OF G_impl_invar])
+    by (metis Kruskal_E_to_G_def carrier_converted_back)
+
+  with Kruskal_Greedy_indep' indep_graph_matroid_expr_3[OF \<open>rbt_inv (Kruskal_Graphs_Matroids.graph_to_edges edge_of G_impl)\<close>]
+    (* \<open>graph_abs.has_no_cycle (Pair_Graph_U_RBT.ugraph_abs (Kruskal_E_to_G carrier_graph_matroid)) G\<close>
+    \<open>Pair_Graph_U_RBT.ugraph_abs G_impl = G\<close>
+    Kruskal_Graphs_Matroids.graph_to_edges_inverse[OF G_impl_invar] *)
+    have "Kruskal_Greedy.indep' (Kruskal_Graphs_Matroids.graph_to_edges edge_of G_impl)" by blast
+  with \<open>rbt_inv (Kruskal_Graphs_Matroids.graph_to_edges edge_of G_impl)\<close>
+    show ?thesis by blast
+qed
+
+
+lemma Kruskal_indep_subset:
+  assumes "rbt_inv X" "rbt_inv Y" "Kruskal_Greedy.indep' X" "rbt_subseteq Y X"
+  shows "Kruskal_Greedy.indep' Y"
+proof-
+  from Kruskal_indep'_eq_has_no_cycle[OF assms(1)] assms(3)
+    have no_cycle: "graph_abs.has_no_cycle (Pair_Graph_U_RBT.ugraph_abs (Kruskal_E_to_G local.carrier_graph_matroid))
+      (Pair_Graph_U_RBT.ugraph_abs (Kruskal_E_to_G X))" by blast
+
+  have X_subset_Y: "Pair_Graph_U_RBT.ugraph_abs (Kruskal_E_to_G Y) \<subseteq>
+    Pair_Graph_U_RBT.ugraph_abs (Kruskal_E_to_G X)" sorry (* TODO HERE *)
+
+  from graph_abs.has_no_cycle_indep_subset[OF carrier_converted_graph_abs no_cycle X_subset_Y]
+    have "graph_abs.has_no_cycle (Pair_Graph_U_RBT.ugraph_abs (Kruskal_E_to_G carrier_graph_matroid))
+      (Pair_Graph_U_RBT.ugraph_abs (Kruskal_E_to_G Y))" by blast
+  with Kruskal_indep'_eq_has_no_cycle[OF \<open>rbt_inv Y\<close>]
+    show ?thesis by blast
+qed
+
+lemma Kruskal_augment:
+  assumes "rbt_inv X" "rbt_inv Y" "Kruskal_Greedy.indep' X" "Kruskal_Greedy.indep' Y" "size X = Suc (size Y)"
+  shows "(\<exists>x. Pair_Graph_U_RBT.isin' x (RBT.diff X Y) \<and> Kruskal_Greedy.indep' (insert_rbt x Y))"
+proof-
+  from Kruskal_indep'_eq_has_no_cycle[OF assms(1)] assms(3)
+    have no_cycle_X: "graph_abs.has_no_cycle (Pair_Graph_U_RBT.ugraph_abs (Kruskal_E_to_G local.carrier_graph_matroid))
+      (Pair_Graph_U_RBT.ugraph_abs (Kruskal_E_to_G X))" by blast
+  from Kruskal_indep'_eq_has_no_cycle[OF assms(2)] assms(4)
+    have no_cycle_Y: "graph_abs.has_no_cycle (Pair_Graph_U_RBT.ugraph_abs (Kruskal_E_to_G local.carrier_graph_matroid))
+      (Pair_Graph_U_RBT.ugraph_abs (Kruskal_E_to_G Y))" by blast
+
+  from Kruskal_Graphs_Matroids.card_graph_to_edges[OF \<open>rbt_inv X\<close>]
+     Kruskal_Graphs_Matroids.card_graph_to_edges[OF \<open>rbt_inv Y\<close>] assms(5)
+
+  have card_rel: "card (Pair_Graph_U_RBT.ugraph_abs (Kruskal_E_to_G X)) = Suc (card (Pair_Graph_U_RBT.ugraph_abs (Kruskal_E_to_G Y))) "
+    unfolding Kruskal_E_to_G_def by metis
+
+  from graph_abs.has_no_cycle_augment[OF carrier_converted_graph_abs no_cycle_X no_cycle_Y card_rel]
+    obtain x where "x \<in> Pair_Graph_U_RBT.ugraph_abs (Kruskal_E_to_G X) - Pair_Graph_U_RBT.ugraph_abs (Kruskal_E_to_G Y)"
+      "graph_abs.has_no_cycle (Pair_Graph_U_RBT.ugraph_abs (local.Kruskal_E_to_G local.carrier_graph_matroid))
+       (Set.insert x (Pair_Graph_U_RBT.ugraph_abs (local.Kruskal_E_to_G Y)))" by blast
+
+  with Kruskal_indep'_eq_has_no_cycle (* TODO HERE !! *)
+  show ?thesis sorry
+qed
+
+
+lemma Kruskal_indep_system_axioms:
+  "Matroid_Specs_Inst.indep_system_axioms carrier_graph_matroid indep_graph_matroid"
+  apply (subst Matroid_Specs_Inst.indep_system_axioms_def)
+  using Kruskal_indep_subset_carrier Kruskal_indep_ex Kruskal_indep_subset by blast
+
+lemma Kruskal_matroid_axioms:
+  "Matroid_Specs_Inst.matroid_axioms carrier_graph_matroid indep_graph_matroid"
+  apply (subst Matroid_Specs_Inst.matroid_axioms_def)
+  using Kruskal_indep_system_axioms Kruskal_augment
+  by blast
+
+end
+
+
+(* thm Kruskal_Greedy.BestInGreedy_correct_1[OF Kruskal_BestInGreedy_axioms] *)
+thm Kruskal_Greedy.BestInGreedy_correct_1[OF Kruskal_BestInGreedy_axioms Kruskal_sort_desc_axioms Kruskal_indep_system_axioms]
+
+(* TODO NOW INSTANTIATE INDEP SYSTEM AXIOMS, CONNECT FINAL THEOREM 
+\<Rightarrow> assumptions on c and order can be left as-is for now *)
+
+
+
+(* !! TODO here assumption !! *)
+(*
+interpretation G_edges_abs: graph_abs
+  where G = "Pair_Graph_U_RBT.ugraph_abs input_G"
+  using Pair_Graph_U_RBT.graph_abs_ugraph[OF pair_graph_u] by simp
+*)
+
+term Kruskal_Greedy.initial_state 
+
+(* TODO define Kruskal_MST, maybe should parametrise with graph and define outside of context? \<Rightarrow> or parametrise
+with c and order? \<Longrightarrow> Don't need to put this function in context, only use use context when pair graph property
+is actually necessary
+\<Rightarrow> maybe parametrise with c and order? *)
+(*
+fun Kruskal_MST :: "(('v::linorder) * ('v rbt)) rbt" where
+  "Kruskal_MST = Kruskal_E_to_G (best_in_greedy_state.result (Kruskal_Greedy.BestInGreedy (Kruskal_Greedy.initial_state c order)))"
+*)
+
+fun Kruskal_MST :: "('e::linorder \<Rightarrow> rat) \<Rightarrow> ('e list) \<Rightarrow> (('v::linorder) * ('v rbt)) rbt" where
+  "Kruskal_MST c order =
+    Kruskal_E_to_G (best_in_greedy_state.result (Kruskal_Greedy.BestInGreedy (Kruskal_Greedy.initial_state c order)))"
+
+context
+  assumes pair_graph_u: "Pair_Graph_U_RBT.pair_graph_u_invar input_G"
+begin
+
+interpretation G_edges_abs: graph_abs
+  where G = "Pair_Graph_U_RBT.ugraph_abs input_G"
+  using Pair_Graph_U_RBT.graph_abs_ugraph[OF pair_graph_u] by simp
+
+(* thm spanning_tree_def *)
+thm G_edges_abs.is_spanning_forest_def
+
+thm Kruskal_Greedy.BestInGreedy_correct_3[OF Kruskal_BestInGreedy_axioms[OF pair_graph_u]
+    Kruskal_sort_desc_axioms Kruskal_indep_system_axioms[OF pair_graph_u]]
+
+lemma Kruskal_correct_final_1:
+  assumes "Kruskal_Greedy.nonnegative c" "Kruskal_Greedy.valid_order order" (* WRONG ASSUMPTIONS !! *)
+  shows "G_edges_abs.is_spanning_forest (Pair_Graph_U_RBT.ugraph_abs (Kruskal_MST c order))"
+  sorry
+
+
+thm Kruskal_matroid_axioms[OF pair_graph_u]
+thm Kruskal_Greedy.BestInGreedy_matroid_iff_opt[OF Kruskal_BestInGreedy_axioms[OF pair_graph_u]
+    Kruskal_sort_desc_axioms Kruskal_indep_system_axioms[OF pair_graph_u]]
+
+term "(Pair_Graph_U_RBT.ugraph_abs (Kruskal_MST c order))"
+lemma Kruskal_correct_final_2:
+  assumes "Kruskal_Greedy.nonnegative c" "Kruskal_Greedy.valid_order order" (* WRONG ASSUMPTIONS !! *)
+    (* introduce new nonnegative predicate, maybe find some way to get order based on existing stuff or assume 
+    function*)
+    "Pair_Graph_U_RBT.pair_graph_u_invar G'"
+    "Pair_Graph_U_RBT.ugraph_abs G' \<subseteq> Pair_Graph_U_RBT.ugraph_abs input_G"
+    "G_edges_abs.is_spanning_forest (Pair_Graph_U_RBT.ugraph_abs G')"
+  (* shows "sum c (Pair_Graph_U_RBT.ugraph_abs (Kruskal_MST c order)) \<le> sum c (Pair_Graph_U_RBT.ugraph_abs G')"  *)
+  shows "True"
+  sorry
+
+(* TODO NOW: JUST GET FINAL THEOREM WORKING, WRITE DOWN CONVERSIONS \<Rightarrow> SORRY THE REST AND MENTION WAS NOT POSSIBLE
+DUE TO TIME CONSTRAINTS *)
+(* IF POSSIBLE: DO REASONING WITH COST FUNCTIONS IN SANDBOX \<Longrightarrow> AT LEAST PUT IT DOWN IN COMMENT MAYBE *)
+
+(*
+TODO NOW:
+CONNECT THMS
+PUT DOWN REASONING WITH COST FUNCTION IN COMMENT
+MAYBE DO ORDER FUNCTION
 
 *)
 
@@ -38,13 +854,41 @@ need smth like
 
 end
 
-(* Should connecting stuff go in separate file + locale? How to do this *)
+end
+
+(* Example: Edge is implemented as pair of vertices where first element is always less than or equal
+to second element *)
+definition edge_of :: "('v::linorder) \<Rightarrow> 'v \<Rightarrow> ('v \<times> 'v)" where
+  "edge_of u v = (if u \<le> v then (u, v) else (v, u))"
+
+definition v1_of :: "('v \<times> 'v) \<Rightarrow> ('v::linorder)" where
+  "v1_of e = fst e"
+
+definition v2_of :: "('v \<times> 'v) \<Rightarrow> ('v::linorder)" where
+  "v2_of e = snd e"
+
+definition "Kruskal_MST' input_G c order = Kruskal_MST input_G v1_of v2_of edge_of c order"
+
+(*
+definition c where "c e = 0"
+
+definition order where "order = []"
+
+value "Kruskal_MST' (Leaf::((nat \<times> nat rbt) rbt)) c order"
+*)
 
 
 
+(* TODO how to instantiate a type as linorder easily using a list? *)
+(* TODO import HOL-Library.Product_Lexorder, then can just use pair as linorder *)
 
+(*
+thm carrier_graph_matroid_def
+thm DFS_Cycles_Interp.initial_state_def
+*)
 
+(* value "DFS_Cycles_state.cycle DFS_Cycles_Interp.initial_state" *)
 
-
+(* value "DFS_Cycles' (\<langle>\<rangle>::((nat \<times> (nat rbt)) rbt)) (\<langle>\<rangle>::(nat rbt))" *)
 
 end
