Spanning_Trees/Graphs_Matroids_Encoding.thy
@@ -1,0 +1,138 @@
+theory Graphs_Matroids_Encoding
+  imports Directed_Set_Graphs.Pair_Graph_U_Specs Matroids_Greedy.Indep_System_Matroids_Specs
+begin
+
+
+(* TODO probably put everything here in locale with proper specs (although probably don't need any
+additional assumptions *)
+
+(* TODO link types properly based on 'v (should we already use uEdge here or just specify arbitrary
+edge type?) \<Rightarrow> Do we even need to "connect" types here? *)
+(* Do we need to specify all of matroid specs with indep function or just the custom set specs? *)
+(* NOTE: !! definitely need either selection function or some sort of foreach which will enable us
+to iterate through the sets !! *)
+
+(* Do we need some assumption on edge type 'e? Or can this be left to the rest of the code? *)
+(* CURRENT IDEA: Define two functions v1_of and v2_of from 'e to 'v which return first and second vertex
+resp., assume additionally that for all edges e, v1_of e and v2_of e return different elements in an axioms
+predicate 
+\<Longrightarrow> ALSO: Assume function edge_of which takes two vertices, with assumption that edge_of a b = edge_of b a
+\<Longrightarrow> maybe can assume that if a \<noteq> b then edge_of a b = edge_of b a? or not?
+*)
+locale Graphs_Matroids_Encoding =
+  pair_graph_u: Pair_Graph_U_Specs where lookup = lookup +
+  matroid: Matroid_Specs where set_insert = set_insert and set_of_sets_isin = set_of_sets_isin
+  for lookup :: "'adj \<Rightarrow> ('v::linorder) \<Rightarrow> 'neighb option" and set_insert :: "('e::linorder) \<Rightarrow> 's \<Rightarrow> 's" and
+    set_of_sets_isin :: "'t \<Rightarrow> 's \<Rightarrow> bool" and adj_fold :: "'adj \<Rightarrow> ('v \<Rightarrow> 'neighb \<Rightarrow> 's \<Rightarrow> 's) \<Rightarrow> 's \<Rightarrow> 's" and
+    neighb_fold :: "'neighb \<Rightarrow> ('v \<Rightarrow> 's \<Rightarrow> 's) \<Rightarrow> 's \<Rightarrow> 's" and set_fold_adj :: "'s \<Rightarrow> ('e \<Rightarrow> 'adj \<Rightarrow> 'adj) \<Rightarrow> 'adj \<Rightarrow> 'adj" and
+    set_fold_neighb :: "'s \<Rightarrow> ('e \<Rightarrow> 'neighb \<Rightarrow> 'neighb) \<Rightarrow> 'neighb \<Rightarrow> 'neighb" +
+  fixes v1_of :: "'e \<Rightarrow> 'v" and v2_of :: "'e \<Rightarrow> 'v" and edge_of :: "'v \<Rightarrow> 'v \<Rightarrow> 'e"
+  (* maybe also do something here related to cost? *)
+  (* TODO WHERE DID I HAVE v1, v2, edge properties ?? \<Longrightarrow> Maybe put this in axioms ? *)
+begin
+
+(* TODO HERE NOW *)
+thm pair_graph_u.pair_graph_u_invar_def
+thm pair_graph_u.graph_inv_def
+thm pair_graph_u.add_edge_def
+
+(* What should invariants be? \<Rightarrow> On one side: pair_graph_u_invar G + neighb_inv V + relationship G V,
+on other side: definitely set_inv, anything else? *)
+
+(* Later just define state and functions, but nothing else *)
+
+(* Iterate through graph itself, then through neighbourhood in nested fashion:
+\<Rightarrow> will have two vertices, form edge_of
+If edge is not in set insert it otherwise don't insert it *)
+fun graph_to_edges :: "'adj \<Rightarrow> 's" where
+  "graph_to_edges G =
+    adj_fold G 
+    (\<lambda>u N E. union E (neighb_fold N 
+        (\<lambda>v E. (let e = (edge_of u v)
+                in (if \<not>(set_isin E e) then set_insert e E else E))) set_empty))
+    set_empty"
+
+(* Iterate through all edges, just use add_edge and v1_of, v2_of from Pair_graph to build a graph, make
+sure every edge is added symmetrically *)
+fun edges_to_graph :: "'s \<Rightarrow> 'adj" where
+  "edges_to_graph E =
+    set_fold_adj E
+    (\<lambda>e G. pair_graph_u.add_edge (pair_graph_u.add_edge G (v1_of e) (v2_of e)) (v2_of e) (v1_of e))
+    empty"
+
+fun edges_to_vertices :: "'s \<Rightarrow> 'neighb" where
+  "edges_to_vertices E = 
+    set_fold_neighb E
+    (\<lambda>e N. if isin N (v1_of e)
+           then (if isin N (v2_of e) then N else insert (v2_of e) N)
+           else (if isin N (v2_of e) then insert (v1_of e) N else insert (v1_of e) (insert (v2_of e) N)))
+    neighb_empty"
+
+(* TODO put down outcommented value theorems (and/or) just note that these functions cannot be
+executed with value since add_edge is a definition, not a fun *)
+
+(* Correctness properties *)
+
+lemma graph_invar_imp_edges_invar:
+  "pair_graph_u.pair_graph_u_invar G \<Longrightarrow> set_inv (graph_to_edges G)"
+  sorry
+
+lemma edges_invar_imp_graph_invar:
+  "set_inv E \<Longrightarrow> pair_graph_u.pair_graph_u_invar (edges_to_graph E)"
+  sorry
+
+lemma edges_invar_imp_vertices_props:
+  assumes "set_inv E"
+  shows "neighb_inv (edges_to_vertices E)"
+    "t_set (edges_to_vertices E) = dVs (pair_graph_u.digraph_abs (edges_to_graph E))"
+  sorry
+
+
+(* probably need invars here additionally, TODO check whether this is the right "direction" *)
+(* lemma
+  "ugraph_abs (edges_to_graph E)" *)
+
+(* If to_set of E1 E2 is the same, ugraph_abs of (edges_to_graph E1) (edges_to_graph E2) is the same *)
+  
+lemma to_set_equal_imp_ugraph_abs_equal:
+  assumes "set_inv X" "set_inv Y" "to_set X = to_set Y"
+  shows "pair_graph_u.ugraph_abs (edges_to_graph X) = pair_graph_u.ugraph_abs (edges_to_graph Y)"
+  sorry
+
+
+lemma graph_to_edges_inverse:
+  "pair_graph_u.pair_graph_u_invar G \<Longrightarrow> edges_to_graph (graph_to_edges G) = G"
+  sorry
+
+lemma edges_to_graph_subset_imp_subset:
+  assumes "set_inv X" "set_inv Y" "pair_graph_u.ugraph_abs (edges_to_graph X) \<subseteq> pair_graph_u.ugraph_abs (edges_to_graph Y)"
+  shows "to_set X \<subseteq> to_set Y"
+  sorry
+
+lemma subset_imp_edges_to_graph_subset:
+  assumes "set_inv X" "set_inv Y" "subseteq X Y"
+  shows "pair_graph_u.ugraph_abs (edges_to_graph X) \<subseteq> pair_graph_u.ugraph_abs (edges_to_graph Y)"
+  sorry
+
+lemma subset_iff_graph_to_edges_subset:
+  assumes "set_inv X" "set_inv Y"
+  shows "subseteq X Y = (pair_graph_u.ugraph_abs (edges_to_graph X) \<subseteq> pair_graph_u.ugraph_abs (edges_to_graph Y))"
+  using edges_to_graph_subset_imp_subset[OF assms] subset_imp_edges_to_graph_subset[OF assms]
+    matroid.set.set_subseteq[OF assms] by blast
+
+(*
+lemma diff_graph_to_edges:
+  assumes "set_inv X" "set_inv Y"
+  shows "diff X Y = pair_graph_u.ugraph_abs (edges_to_graph X) - pair_graph_u.ugraph_abs (edges_to_graph Y)"
+  sorry
+*)
+
+lemma card_graph_to_edges:
+  assumes "set_inv X"
+  shows "cardinality X = card (pair_graph_u.ugraph_abs (edges_to_graph X))"
+  sorry
+
+end
+
+
+end
