Spanning_Trees/Spanning_Trees.thy
@@ -1034,6 +1034,10 @@ if yes, then continue with cycle check, otherwise return false
 
 end
 
+lemma ex_graph_impl_ugraph_abs:
+  "graph_abs G \<Longrightarrow> \<exists>G_impl. pair_graph_u_invar G_impl \<and> ugraph_abs G_impl = G"
+  sorry
+
 end
 
 
